\documentclass[11pt]{article}
\usepackage{minted}
\usepackage{amsfonts, amssymb, amsmath, float}
\usepackage{enumerate, esint, nicefrac, algorithm2e}
\parindent 0px
\date{September 9, 2022}
\title{MATH210 :\hspace{2px}: Homework 1}
\author{Ryan Magdaleno}

% Helpful ::
% \line(1,0){358px}

\begin{document}
\maketitle

%%%%%%%%%%%%%%%%%%%%%%%%%%%%%%%%%%%%%%%%%%%%%%%%%%%%%%%%%%%%%%%%%%%%%%%%%%%%%%%%%%%%%%%%%

\textbf{Problem 1.}
$$\text{Let }u = \langle2,1,-1\rangle\text{ and }v=\langle1,2,1\rangle.$$
\vspace{5px}\textbf{Solution ::}
\begin{enumerate}[a)]
\item 
\begin{align}
    \text{proj}_vu &= \left(\frac{u\cdot v}{|v|^2}\right)\cdot v \\
    w &= \left(\frac{2(1)+1(2)-1(1)}{\left(\sqrt{1^2+2^2+1^2}\right)^2}\right)
    \cdot \langle1,2,1\rangle \\
    w &= \frac{3}{6}\langle1,2,1\rangle = \frac{1}{2}\langle1,2,1\rangle \\
    w &= \left\langle\frac{1}{2},1,\frac{1}{2}\right\rangle
\end{align}
\item
$u-w$ or $u+(-w)$:
\begin{align}
    \langle2,1,-1\rangle &- \left\langle\frac{1}{2},1,\frac{1}{2}\right\rangle \\
    u-w &= \langle1.5,0,-1.5\rangle
\end{align}
\item 
Show that $u-w$ is orthagonal to $v$.
$$u-w\cdot v = 1.5(1)+0(2)-1.5(1) = 0$$
$\therefore u-w$ and $v$ are orthagonal. 
\pagebreak

\item
Write $v$ as the sum of orthagonal perp. to $v$.
\begin{align}
    u_1 &= u_1 + u_2 = \text{proj}_vu + (u-\text{proj}_vu) \\
    u_1 &= \left(\frac{u\cdot v}{v\cdot v}\right)\cdot v = \langle0.5,1,0.5\rangle \\
    u_2 &= \langle2,1,-1\rangle - \langle0.5,1,0.5\rangle \\
    u_2 &= \langle1.5, 0, -1.5\rangle \\
    u &= \langle0.5,1,0.5\rangle + \langle1.5,0,-1.5\rangle \\
    u &= \langle2,1,-1\rangle
\end{align}

\end{enumerate}
\pagebreak

%%%%%%%%%%%%%%%%%%%%%%%%%%%%%%%%%%%%%%%%%%%%%%%%%%%%%%%%%%%%%%%%%%%%%%%%%%%%%%%%%%%%%%%%%

\textbf{Problem 2.}
$$|u| = 1, |v| = 3, u\cdot v = -2$$
\vspace{5px}\textbf{Solution ::}
\begin{enumerate}[a)]
\item 
\begin{align}
    |u + v| &= \sqrt{|u+v|^2} \\
    &= \sqrt{|u|^2 + u\cdot v+u\cdot v+|v|^2} \\
    &= \sqrt{1^2 + (-2)+(-2)+3^2} \\
    |u+v| &= \sqrt{6}
\end{align}

\item $||(u+2v)\times v||$
\begin{align}
    |u+2v| &= \sqrt{|u|^2+u\cdot 2v+u\cdot2v+2|v|^2} \\
    &= \sqrt{1^2 + (-2) + (-2) + 18} \\
    &= \sqrt{15}
\end{align}
\end{enumerate}

\end{document}